theories/imp_to_asm_compiler.v
@@ -12,16 +12,59 @@ Require Import refframe.imp.
 Require Import refframe.asm.
 Require Import refframe.imp_to_asm.
 
+
 Local Open Scope Z_scope.
 
-Section theorems.
-Context `{FinMap K M}.
-Lemma insert_subseteq_Some {A} (m1 m2 : M A) i x :
-  <[i:=x]> m1 ⊆ m2 → m2 !! i = Some x.
-Proof. intros Hsub. eapply lookup_weaken; [|done]. apply lookup_insert. Qed.
-End theorems.
-
 Set Default Proof Using "Type".
+(*
+optimizations:
+
+fn f() :=
+  local x
+  x ← 1;
+  g(!x + !x);
+  x ← 2;
+  return !x
+
+optimize to:
+
+fn f() :=
+  let x := 1;
+  g(x + x);
+  let x := 2;
+  return x
+
+1 + 1 → 2
+
+if 1 then e1 else e2
+->
+e1
+
+
+compilation chain:
+
+1. make let-names unique (each name is only assigned once)
+2. translate nested expressions to linear expressions
+3. optimize linear
+3.1. propagate values and let-bindings
+3.2. reuse dead let-names
+4. translate to asm
+
+*)
+
+Lemma list_elem_of_weaken {A} (xs ys : list A) x:
+  x ∈ xs → xs ⊆ ys → x ∈ ys.
+Proof. set_solver. Qed.
+
+Lemma list_subseteq_cons_l {A} x (xs ys : list A):
+  x ∈ ys → xs ⊆ ys → x :: xs ⊆ ys.
+Proof. set_solver. Qed.
+
+Transparent map_preserved.
+Lemma map_preserved_app {K A} `{Countable K} ns1 ns2 (m m' : gmap K A) :
+  map_preserved (ns1 ++ ns2) m m' ↔ map_preserved ns1 m' m ∧ map_preserved ns2 m' m.
+Proof. unfold map_preserved. set_solver. Qed.
+Opaque map_preserved.
 
 Lemma deep_to_asm_instrs_nil pc :
   deep_to_asm_instrs pc [] = ∅.
@@ -29,6 +72,16 @@ Proof. done. Qed.
 Lemma deep_to_asm_instrs_cons pc di dins :
   deep_to_asm_instrs pc (di :: dins) = <[pc := deep_to_asm_instr di]> $ deep_to_asm_instrs (pc + 1) dins.
 Proof. done. Qed.
+
+Lemma deep_to_asm_instrs_cons_inv pc di dins ins :
+  deep_to_asm_instrs pc (di :: dins) ⊆ ins →
+  ins !! pc = Some (deep_to_asm_instr di) ∧ deep_to_asm_instrs (pc + 1) dins ⊆ ins.
+Proof.
+  rewrite deep_to_asm_instrs_cons => Hsub.
+  split.
+  - eapply lookup_weaken; [|done]. apply lookup_insert.
+  - etrans; [|done]. apply insert_subseteq. apply lookup_map_seqZ_None. lia.
+Qed.
 
 Inductive i2a_error :=
 | UnsupportedExpr (e : expr)
@@ -64,47 +117,55 @@ Definition variable_registers : list string :=
   ["R19"; "R20"; "R21"; "R22"; "R23"; "R24"; "R25"; "R26"; "R27"; "R28"; "R29"].
 
 Inductive place :=
-| PReg (r : string) | PStack (slot : Z).
+| PReg (r : string) | PStack (slot : N).
 
 Record state := State {
   s_f2i : gmap string Z;
-  s_stacksize : Z;
+  s_stacksize : N;
   s_places : gmap string place;
-  s_saved_registers : list (string * Z);
+  s_saved_registers : list (string * N);
   s_sp_above : bool; (* tracks whether sp currently points to above the stack or below *)
 }.
 Global Instance eta_state : Settable _ := settable! State <s_f2i; s_stacksize; s_places; s_saved_registers; s_sp_above>.
 Add Printing Constructor state.
 
+Definition s_stack_places (s : gmap string place) : list N :=
+  omap (λ '(_, p), if p is PStack slot then Some slot else None) (map_to_list s).
+
+Lemma s_stack_places_insert s a p :
+  s !! a = None →
+  s_stack_places (<[a:=p]> s) ≡ₚ (if p is PStack slot then [slot] else []) ++ (s_stack_places s).
+Proof. move => ?. rewrite /s_stack_places map_to_list_insert //; csimpl. by destruct p. Qed.
+
 Definition initial_state (f2i : gmap string Z) : state := State f2i 0 ∅ [] true.
 
 Definition M := compiler_monad state (list_compiler_monoid deep_asm_instr) i2a_error.
 
-Definition alloc_stack : M Z :=
+Definition alloc_stack : M N :=
   s ← cget;
   cassert (AssertionFailed "alloc_stack: s_sp_above is not true") (s.(s_sp_above) = true);;
-  cput (s <| s_stacksize := s.(s_stacksize) + 1 |>);;
+  cput (s <| s_stacksize := (s.(s_stacksize) + 1)%N |>);;
   mret s.(s_stacksize).
 
 Definition move_sp (above : bool) : M unit :=
   s ← cget;
   cassert (AssertionFailed "move_sp: already at the right place") (s.(s_sp_above) ≠ above);;
-  cappend [Aadd "SP" "SP" (ImmediateOp $ if s.(s_sp_above) then - s.(s_stacksize) else s.(s_stacksize))];;
+  cappend [Aadd "SP" "SP" (ImmediateOp $ if s.(s_sp_above) then - Z.of_N s.(s_stacksize) else Z.of_N s.(s_stacksize))];;
   cput (s <| s_sp_above := above |>);;
   mret tt.
 
 (* for stack slot [slot] returns offset that one needs to add to SP to
 reach the slot *)
-Definition stack_offset (slot : Z) : M Z :=
+Definition stack_offset (slot : N) : M Z :=
   s ← cget;
-  mret ((if s.(s_sp_above) then 0 else s.(s_stacksize)) - slot - 1).
+  mret ((if s.(s_sp_above) then 0 else Z.of_N s.(s_stacksize)) - Z.of_N slot - 1).
 
-Definition read_stack (r : string) (slot : Z) : M unit :=
+Definition read_stack (r : string) (slot : N) : M unit :=
   o ← stack_offset slot;
   cappend [Aload r "SP" o];;
   mret tt.
 
-Definition write_stack (r : string) (slot : Z) : M unit :=
+Definition write_stack (r : string) (slot : N) : M unit :=
   o ← stack_offset slot;
   cappend [Astore r "SP" o];;
   mret tt.
@@ -157,7 +218,6 @@ Fixpoint allocate_places (ns : list string) (regs : list string) : M unit :=
   end.
 
 Definition initialize_args (args : list string) : M unit :=
-  s ← cget;
   cmap args 0 (λ n a,
     r ← cassert_opt TooManyArgs (args_registers !! n);
     write_var r a);;
@@ -184,63 +244,56 @@ Definition read_operand (r : string) (e : expr) : M unit :=
   | _ => cerror (UnknownOperand e)
   end.
 
-Fixpoint translate_expr (e : expr) : M unit :=
+Definition translate_expr_op (e : expr) : M unit :=
   match e with
   | Val v => read_operand "R0" (Val v)
   | Var v => read_operand "R0" (Var v)
-  | LetE v (Val v1) e =>
-      read_operand "R0" (Val v1);;
-      write_var "R0" v;;
-      translate_expr e
-  | LetE v (Var v1) e =>
-      read_operand "R0" (Var v1);;
-      write_var "R0" v;;
-      translate_expr e
-  | LetE v (BinOp v1 op v2) e =>
-      read_operand "R0" v1;;
-      read_operand "R1" v2;;
+  | BinOp v1 op v2 =>
+      read_operand "R1" v1;;
+      read_operand "R2" v2;;
       match op with
-      | AddOp | ShiftOp => cappend [Aadd "R2" "R0" (RegisterOp "R1")]
-      | EqOp => cappend [Aseq "R2" "R0" (RegisterOp "R1")]
-      | LeOp => cappend [Asle "R2" "R0" (RegisterOp "R1")]
-      | LtOp => cappend [Aslt "R2" "R0" (RegisterOp "R1")]
-      end;;
-      write_var "R2" v;;
-      translate_expr e
-  | LetE v (Load v1) e =>
-      read_operand "R0" v1;;
-      cappend [Aload "R1" "R0" 0];;
-      write_var "R1" v;;
-      translate_expr e
-  | LetE v (Store v1 v2) e =>
-      read_operand "R0" v1;;
-      read_operand "R1" v2;;
-      cappend [Astore "R1" "R0" 0];;
-      write_var "R1" v;;
-      translate_expr e
-  (* We cannot handle [LetE v (If v1 e2 e3) e] because e2 and e3 could
-  contain let bindings whose effect we would need to undo before
-  executing e. Instead we rewrite LetE v (If v1 e2 e3) e to If v1
-  (LetE v e2 e) (LetE v e3 e). *)
-  | If v1 e2 e3 =>
-      read_operand "R0" v1;;
-      '(_, a1) ← cscope (translate_expr e2);
-      '(_, a2) ← cscope (translate_expr e3);
-      (* + 1 for the branch_eq at the start and + 1 for the branch at the end *)
-      cappend [Abranch_eq false (ImmediateOp (2 + length a1)) "R0" (ImmediateOp 0)];;
-      cappend a1;;
-      cappend [Abranch false (ImmediateOp (1 + length a2))];;
-      cappend a2
-  | LetE v (Call f vs) e =>
+      | AddOp | ShiftOp => cappend [Aadd "R0" "R1" (RegisterOp "R2")]
+      | EqOp => cappend [Aseq "R0" "R1" (RegisterOp "R2")]
+      | LeOp => cappend [Asle "R0" "R1" (RegisterOp "R2")]
+      | LtOp => cappend [Aslt "R0" "R1" (RegisterOp "R2")]
+      end
+  | Load v1 =>
+      read_operand "R1" v1;;
+      cappend [Aload "R0" "R1" 0]
+  | Store v1 v2 =>
+      read_operand "R1" v1;;
+      read_operand "R0" v2;;
+      cappend [Astore "R0" "R1" 0]
+  | Call f vs =>
       s ← cget;
       a ← cassert_opt (UnknownFunction f) (s.(s_f2i) !! f);
       cmap vs 0 (λ n a,
         r ← cassert_opt TooManyArgs (args_registers !! n);
         read_operand r a);;
-      cappend [Abranch_link true (ImmediateOp a)];;
+      cappend [Abranch_link true (ImmediateOp a)]
+  | _ => cerror (UnsupportedExpr e)
+  end.
+
+Fixpoint translate_expr (e : expr) : M unit :=
+  match e with
+  | LetE v e1 e =>
+      translate_expr_op e1;;
       write_var "R0" v;;
       translate_expr e
-  | _ => cerror (UnsupportedExpr e)
+  (* We cannot handle [LetE v (If v1 e2 e3) e] because e2 and e3 could
+  contain let bindings whose effect we would need to undo before
+  executing e. Instead we rewrite LetE v (If v1 e2 e3) e to If v1
+  (LetE v e2 e) (LetE v e3 e). *)
+  | If e1 e2 e3 =>
+      translate_expr_op e1;;
+      '(_, a2) ← cscope (translate_expr e2);
+      '(_, a3) ← cscope (translate_expr e3);
+      (* + 1 for the branch_eq at the start and + 1 for the branch at the end *)
+      cappend [Abranch_eq false (ImmediateOp (2 + length a2)) "R0" (ImmediateOp 0)];;
+      cappend a2;;
+      cappend [Abranch false (ImmediateOp (1 + length a3))];;
+      cappend a3
+  | _ => translate_expr_op e
   end.
 
 Definition pass (fn : fndef) : M unit :=
@@ -257,7 +310,7 @@ Definition pass (fn : fndef) : M unit :=
 Definition test_fn : fndef := {|
   fd_args := ["a"; "b"];
   fd_body := LetE "r" (BinOp (Var "a") AddOp (Var "b")) $
-             Var "r";
+             BinOp (Var "a") AddOp (Var "r");
   fd_static := I
 |}.
 
@@ -288,68 +341,64 @@ Class ProofFixedValues := {
   pf_fns : gmap string fndef;
   pf_cs : list imp_to_asm_stack_item;
   pf_rsold : gmap string Z;
+  pf_f2i : gmap string Z;
 }.
 
 Section proof.
 Context `{!ProofFixedValues}.
 
 (** general invariants *)
-Definition stack_slot (slot : Z) (v : Z) : uPred _ :=
-  ⌜0 ≤ slot⌝ ∗ i2a_mem_constant (pf_sp - slot - 1) v.
+Definition stack_slot (slot : N) (v : Z) : uPred _ :=
+  i2a_mem_constant (pf_sp - Z.of_N slot - 1) v.
 
 Definition ci2a_regs_inv (s : state) (lr rs : gmap string Z) : uPred imp_to_asmUR :=
   ⌜pf_rsold !! "SP" = Some pf_sp⌝ ∗
-  ⌜rs !! "SP" = Some (if s.(s_sp_above) then pf_sp else pf_sp - s.(s_stacksize))⌝ ∗
+  ⌜rs !! "SP" = Some (if s.(s_sp_above) then pf_sp else pf_sp - Z.of_N s.(s_stacksize))⌝ ∗
   ⌜map_scramble touched_registers lr rs⌝ ∗
-  ⌜map_list_included tmp_registers rs⌝ ∗
-  ⌜map_list_included saved_registers rs⌝.
-
-Definition ci2a_mem_inv (stacksize : Z) (mem : gmap Z Z) : uPred imp_to_asmUR :=
-  ∃ amem, ⌜0 ≤ stacksize⌝ ∗ ⌜i2a_mem_agree mem amem⌝ ∗ ⌜i2a_mem_sp (pf_sp - stacksize) amem⌝ ∗ i2a_mem_auth amem.
-
-Definition ci2a_heap_inv (h : heap_state) : uPred imp_to_asmUR :=
-  ∃ ih, ⌜i2a_heap_agree h ih⌝ ∗ i2a_heap_shared_agree (h_heap h) ih ∗ i2a_heap_auth ih.
+  ⌜map_list_included touched_registers rs⌝ ∗
+  ⌜s.(s_f2i) = pf_f2i⌝.
 
 Definition ci2a_inv (s : state) (lr rs : gmap string Z) (mem : gmap Z Z) (h : heap_state) : uPred _ :=
-    ci2a_mem_inv s.(s_stacksize) mem ∗
-    ci2a_heap_inv h ∗
+    i2a_mem_inv (pf_sp - Z.of_N s.(s_stacksize)) mem ∗
+    i2a_heap_inv h ∗
     ci2a_regs_inv s lr rs.
 
 (** lemmas for general invariants *)
-Lemma mem_constant_update v' a v mem ss:
-  i2a_mem_constant a v -∗
-  ci2a_mem_inv ss mem ==∗
-  i2a_mem_constant a v' ∗ ci2a_mem_inv ss (<[a := v']>mem).
-Proof.
-  iIntros "Hconst".
-  iDestruct 1 as (?? Hag Hsp) "Hauth".
-  iDestruct (i2a_mem_lookup with "[$] [$]") as %?.
-  iMod (i2a_mem_update with "[$]") as "[? $]". iModIntro.
-  iExists _. iFrame. iPureIntro. split!.
-  - move => ?? /lookup_insert_Some[[??]|[??]]; simplify_map_eq'; [done|]. by apply Hag.
-  - move => ??. apply lookup_insert_None. unfold i2a_mem_sp in *. naive_solver lia.
-Qed.
-
-Lemma stack_slot_update v' slot v mem ss:
+Lemma stack_slot_lookup slot v mem sp:
   stack_slot slot v -∗
-  ci2a_mem_inv ss mem ==∗
-  stack_slot slot v' ∗ ci2a_mem_inv ss (<[pf_sp - slot - 1:=v']>mem).
-Proof. iIntros "(%&?) ?". iMod (mem_constant_update with "[$] [$]") as "[$ $]". by iModIntro. Qed.
+  i2a_mem_inv sp mem -∗
+  ⌜mem !!! (pf_sp - Z.of_N slot - 1) = v⌝.
+Proof. iIntros "? ?". iApply (i2a_mem_lookup with "[$] [$]"). Qed.
+
+Lemma stack_slot_update v' slot v mem sp:
+  stack_slot slot v -∗
+  i2a_mem_inv sp mem ==∗
+  stack_slot slot v' ∗ i2a_mem_inv sp (<[pf_sp - Z.of_N slot - 1:=v']>mem).
+Proof. iIntros "? ?". iMod (i2a_mem_update with "[$] [$]") as "[$ $]". by iModIntro. Qed.
 
 Lemma stack_slot_alloc mem ss:
-  ci2a_mem_inv ss mem ==∗
-  ∃ v, stack_slot ss v ∗ ci2a_mem_inv (ss + 1) mem.
+  i2a_mem_inv (pf_sp - Z.of_N ss) mem ==∗
+  ∃ v, stack_slot ss v ∗ i2a_mem_inv (pf_sp - Z.of_N (ss + 1)) mem.
 Proof.
-  iDestruct 1 as (? ? Hag Hsp) "Hauth".
-  iMod (i2a_mem_alloc (pf_sp - ss - 1) with "[$]") as "[? ?]". { apply Hsp. lia. } iModIntro.
-  iExists _. iFrame. iSplit; [done|]. iExists _. iFrame. iPureIntro. split!.
-  - lia.
-  - move => ?? /lookup_insert_Some[[??]|[??]]; simplify_map_eq => //. by apply Hag.
-  - move => ??. apply lookup_insert_None. split; [|lia]. apply Hsp. lia.
+  iIntros "?".
+  iMod (i2a_mem_alloc with "[$]") as "[??]". iModIntro.
+  iExists _. iFrame.
+  by have -> : (pf_sp - Z.of_N ss - 1) = (pf_sp - Z.of_N (ss + 1)) by lia.
+Qed.
+
+Lemma ci2a_regs_inv_mono_insert rs s r lr v :
+  r ∈ touched_registers ∧ r ≠ "SP" →
+  ci2a_regs_inv s lr rs -∗
+  ci2a_regs_inv s lr (<[r := v]> rs).
+Proof.
+  iIntros ([??] (?&?&?&?&?)).
+  iPureIntro. simplify_map_eq. split!.
+  - by apply map_scramble_insert_r_in.
+  - by apply map_list_included_insert.
 Qed.
 
 (** ci2a_places_inv *)
-Definition ci2a_places_inv (ps : gmap string place) (sr : list (string*Z)) (vs : gmap string val) (rs : gmap string Z)
+Definition ci2a_places_inv (ps : gmap string place) (sr : list (string*N)) (vs : gmap string val) (rs : gmap string Z)
   : uPred imp_to_asmUR :=
   ([∗ map] n↦p∈ps, ∃ av,
      (if vs !! n is Some v then imp_val_to_asm_val v av else True) ∗
@@ -358,14 +407,16 @@ Definition ci2a_places_inv (ps : gmap string place) (sr : list (string*Z)) (vs :
      | PStack slot => stack_slot slot av
      end) ∗
    ([∗ list] r∈sr, ∃ v, ⌜pf_rsold !! r.1 = Some v⌝ ∗ stack_slot r.2 v) ∗
-   ⌜Forall (λ v, v ∈ sr.*1 ∨ pf_rsold !! v = rs !! v) variable_registers⌝.
+   ⌜sr.*1 ⊆ "R30"::variable_registers⌝ ∗
+   ⌜Forall (λ v, v ∈ sr.*1 ∨ pf_rsold !! v = rs !! v) variable_registers⌝ ∗
+   ⌜∀ v1 v2 r, ps !! v1 = Some (PReg r) → ps !! v2 = Some (PReg r) → v1 = v2⌝.
 
 Lemma ci2a_places_inv_mono_rs rs ps sr vs rs' :
   map_preserved variable_registers rs rs' →
   ci2a_places_inv ps sr vs rs -∗
   ci2a_places_inv ps sr vs rs'.
 Proof.
-  iIntros (Hp) "(Hp&$&%Hv)".
+  iIntros (Hp) "(Hp&$&$&%Hv&$)".
   iSplitL "Hp".
   - iApply (big_sepM_impl with "[$]"). iIntros "!>" (???). iDestruct 1 as (?) "[? Hp]".
     iExists _. iFrame. case_match => //. iDestruct "Hp" as %(?&?&?). iPureIntro. split!.
@@ -383,6 +434,10 @@ Definition sim (n : trace_index) (b : bool) (dins : list deep_asm_instr) (e : ex
   iSat_end (AsmState (Some []) rs mem pf_ins
              ⪯{asm_module, imp_to_asm (dom _ pf_ins) (dom _ pf_fns) s.(s_f2i) imp_module, n, b}
            (SMProg, Imp e h pf_fns, (PPInside, I2A pf_cs lr, rf))).
+
+Lemma to_sim n b dins e s rs :
+  sim n b dins e s rs -∗ sim n b dins e s rs.
+Proof. done. Qed.
 
 Lemma sim_mono_s n b dins e s s' rs:
   (∀ lr mem h,
@@ -405,7 +460,7 @@ Proof.
 Qed.
 
 Lemma sim_get_sp s p b n rs e:
-  (⌜rs !! "SP" = Some (if s.(s_sp_above) then pf_sp else pf_sp - s.(s_stacksize))⌝ -∗ sim n b p e s rs) -∗
+  (⌜rs !! "SP" = Some (if s.(s_sp_above) then pf_sp else pf_sp - Z.of_N s.(s_stacksize))⌝ -∗ sim n b p e s rs) -∗
   sim n b p e s rs.
 Proof.
   iIntros "Hcont" (?????) "Hrf (?&?&(?&%&?))".
@@ -414,46 +469,70 @@ Proof.
 Qed.
 
 Lemma sim_regs_included s p b n rs e:
-  (⌜map_list_included tmp_registers rs⌝ -∗ ⌜map_list_included saved_registers rs⌝ -∗ sim n b p e s rs) -∗
+  (⌜map_list_included touched_registers rs⌝ -∗ sim n b p e s rs) -∗
   sim n b p e s rs.
 Proof.
   iIntros "Hcont" (?????) "Hrf (?&?&(?&?&%))".
-  iApply ("Hcont" with "[] [] [//] Hrf"); [naive_solver..|].
+  iApply ("Hcont" with "[] [//] Hrf"); [naive_solver..|].
   by iFrame.
 Qed.
 
+Lemma sim_Amov r o n b p' e rs s :
+  r ∈ touched_registers ∧ r ≠ "SP" ∧ r ≠ "PC" →
+  sim n true p' e s (<["PC" := rs !!! "PC" + 1]> $ <[r := op_lookup rs o]>rs) -∗
+  sim n b (Amov r o :: p') e s rs.
+Proof.
+  iIntros ([?[??]]) "Hcont".
+  iApply sim_regs_included. iIntros (?).
+  iIntros (???? Hins) "Hrf Hinv". iSatStop.
+  tstep_i => ??. simplify_map_eq'.
+  move: Hins => /deep_to_asm_instrs_cons_inv[??]. simplify_map_eq.
+  rewrite orb_true_r.
+  tstep_i. split!. { apply: map_list_included_is_Some; [done|]. naive_solver. }
+  tstep_i. simplify_map_eq'. split!.
+  iSatStart. iApply ("Hcont" with "[] Hrf"). { by simplify_map_eq'. }
+  iDestruct "Hinv" as "(?&?&?)". iFrame.
+  iApply ci2a_regs_inv_mono_insert; [compute_done|].
+  by iApply ci2a_regs_inv_mono_insert.
+Qed.
+
+Lemma sim_Var s p b n rs e K v `{!ImpExprFill e K (Var v)}:
+  ⊢ sim n b p e s rs.
+Proof.
+  destruct ImpExprFill0; subst.
+  iIntros (?????) "??". iSatStop. by tstep_s.
+Qed.
+
 (** rules for operations *)
-Lemma write_stack_correct s s' p p' r res b n slot rs v v' e:
-  crun s (write_stack r slot) = CResult s' p (CSuccess res) →
-  rs !! r = Some v' →
-  stack_slot slot v -∗
-  (⌜s' = s⌝ -∗ stack_slot slot v' -∗ sim n true p' e s' (<["PC" := rs !!! "PC" + length p]> rs)) -∗
+Lemma move_sp_correct s s' p p' r n b e rs ab:
+  crun s (move_sp ab) = CResult s' p (CSuccess r) →
+  (∀ pc' sp', ⌜s' = s <|s_sp_above := ab |>⌝ -∗
+        sim n true p' e s' (<["PC":=pc']> $ <["SP":=sp']>rs)) -∗
   sim n b (p ++ p') e s rs.
 Proof.
-  unfold write_stack, stack_offset.
-  iIntros (??) "Hs Hcont". simplify_crun_eq.
+  unfold move_sp. move => ?. simplify_crun_eq. iIntros "Hcont".
   iApply sim_get_sp. iIntros (?).
-
-  iIntros (?????) "Hrf (Hmem&Hheap&Hregs)". iSatStop.
+  iIntros (???? Hins) "Hrf (Hmem&Hheap&Hregs)".
+  iSatStop.
   tstep_i => ??. simplify_map_eq'.
-  rewrite deep_to_asm_instrs_cons in H2.
-  move: (H2) => Hsub.
-  apply insert_subseteq_Some in Hsub. simplify_option_eq.
+  move: Hins => /deep_to_asm_instrs_cons_inv[??]. simplify_map_eq.
   rewrite orb_true_r.
-
   tstep_i. split!.
-  tstep_i. split!. simplify_map_eq'.
-  iSatStartBupd.
-  iMod (stack_slot_update with "[$] [$]") as "[??]". iModIntro.
-  iApply ("Hcont" with "[//] [$] [%] Hrf").
-  - simplify_map_eq'. admit.
-  - iFrame.
-    admit.
-Admitted.
+  tstep_i. split!; simplify_map_eq'; [done|].
+  iSatStart.
+  iApply ("Hcont" with "[//] [] Hrf"). { by simplify_map_eq'. }
+  iFrame.
+  iDestruct "Hregs" as %(?&?&?&?&?).
+  iApply ci2a_regs_inv_mono_insert; [compute_done|].
+  iPureIntro. simplify_map_eq. split!.
+  - by repeat case_match; f_equal; lia.
+  - apply map_scramble_insert_r_in; [compute_done|done].
+  - by apply map_list_included_insert.
+Qed.
 
 Lemma alloc_stack_correct s s' p p' r n b e rs:
   crun s alloc_stack = CResult s' p (CSuccess r) →
-  (∀ v, ⌜s' = s <|s_stacksize := (s.(s_stacksize) + 1)%Z |>⌝ -∗
+  (∀ v, ⌜s' = s <|s_stacksize := (s.(s_stacksize) + 1)%N |>⌝ -∗
         ⌜r = s.(s_stacksize)⌝ -∗
         ⌜p = []⌝ -∗
         stack_slot s.(s_stacksize) v -∗
@@ -469,6 +548,178 @@ Proof.
   iPureIntro. split!. by case_match.
 Qed.
 
+Lemma read_stack_correct s s' p p' r res b n slot rs v e:
+  crun s (read_stack r slot) = CResult s' p (CSuccess res) →
+  r ∈ touched_registers ∧ r ≠ "SP" ∧ r ≠ "PC" →
+  stack_slot slot v -∗
+  (⌜s' = s⌝ -∗ stack_slot slot v -∗ sim n true p' e s' (<["PC" := rs !!! "PC" + length p]> $ <[r := v]> rs)) -∗
+  sim n b (p ++ p') e s rs.
+Proof.
+  unfold read_stack, stack_offset.
+  iIntros (?[?[??]]) "Hs Hcont". simplify_crun_eq.
+  iApply sim_get_sp. iIntros (?).
+  iApply sim_regs_included. iIntros (?).
+
+  iIntros (???? Hins) "Hrf (Hmem&Hheap&Hregs)". iSatStop.
+  tstep_i => ??. simplify_map_eq'.
+  move: Hins => /deep_to_asm_instrs_cons_inv[??]. simplify_map_eq.
+  rewrite orb_true_r.
+  tstep_i. split!. { apply: map_list_included_is_Some; [done|]. naive_solver. }
+  tstep_i. split!; simplify_map_eq'; [done|].
+  iSatStart.
+  iDestruct (stack_slot_lookup with "[$] [$]") as %?. simplify_eq.
+  have -> : (if s_sp_above s then pf_sp else pf_sp - Z.of_N (s_stacksize s)) +
+       ((if s_sp_above s then 0 else Z.of_N (s_stacksize s)) - Z.of_N slot - 1) = pf_sp - Z.of_N slot - 1 by case_match; lia.
+  iApply ("Hcont" with "[//] [$] [%] Hrf"). { by simplify_map_eq'. } iFrame.
+  iApply ci2a_regs_inv_mono_insert; [compute_done| ].
+  by iApply ci2a_regs_inv_mono_insert.
+Qed.
+
+Lemma write_stack_correct s s' p p' r res b n slot rs v v' e:
+  crun s (write_stack r slot) = CResult s' p (CSuccess res) →
+  rs !! r = Some v' →
+  stack_slot slot v -∗
+  (⌜s' = s⌝ -∗ stack_slot slot v' -∗ sim n true p' e s' (<["PC" := rs !!! "PC" + length p]> rs)) -∗
+  sim n b (p ++ p') e s rs.
+Proof.
+  unfold write_stack, stack_offset.
+  iIntros (??) "Hs Hcont". simplify_crun_eq.
+  iApply sim_get_sp. iIntros (?).
+
+  iIntros (???? Hins) "Hrf (Hmem&Hheap&Hregs)". iSatStop.
+  tstep_i => ??. simplify_map_eq'.
+  move: Hins => /deep_to_asm_instrs_cons_inv[??]. simplify_map_eq.
+  rewrite orb_true_r.
+  tstep_i. split!.
+  tstep_i. split!. simplify_map_eq'.
+  iSatStartBupd.
+  iMod (stack_slot_update with "[$] [$]") as "[??]". iModIntro.
+  iApply ("Hcont" with "[//] [$] [%] Hrf"). { by simplify_map_eq'. }
+  have -> : (if s_sp_above s then pf_sp else pf_sp - Z.of_N (s_stacksize s)) +
+       ((if s_sp_above s then 0 else Z.of_N (s_stacksize s)) - Z.of_N slot - 1) = pf_sp - Z.of_N slot - 1 by case_match; lia.
+  iFrame.
+  iApply ci2a_regs_inv_mono_insert; [compute_done|done].
+Qed.
+
+Lemma read_var_correct s s' p p' r res b n rs v v' e vs:
+  crun s (read_var r v) = CResult s' p (CSuccess res) →
+  r ∈ tmp_registers ∧ r ≠ "PC" →
+  vs !! v = Some v' →
+  ci2a_places_inv s.(s_places) s.(s_saved_registers) vs rs -∗
+  (∀ pc' av,
+   let rs' := (<["PC":=pc']> $ <[r := av]>rs) in
+   ⌜s' = s⌝ -∗
+   imp_val_to_asm_val v' av -∗
+   ci2a_places_inv s.(s_places) s.(s_saved_registers) vs rs' -∗
+   sim n true p' e s' rs') -∗
+  sim n b (p ++ p') e s rs.
+Proof.
+  unfold read_var.
+  iIntros (?[Hin ?]?) "Hp Hcont". simplify_crun_eq.
+  have ? : r ∈ touched_registers ∧ r ≠ "SP" ∧ r ≠ "PC". {
+    split. 2: split => ?; subst; set_solver.
+    apply: (list_elem_of_weaken tmp_registers); [done| ].
+    clear. set_unfold. naive_solver.
+  }
+  iDestruct "Hp" as "[Hp ?]".
+  iDestruct (big_sepM_lookup_acc with "Hp") as "[[% [Hv Hpl]] Hp]"; [done|]. simplify_map_eq.
+  iDestruct "Hv" as "#Hv".
+  case_match; simplify_crun_eq.
+  - iDestruct "Hpl" as %(?&?&?).
+    iApply sim_Amov; [done|].
+    simplify_map_eq'.
+    iApply ("Hcont" with "[//] Hv").
+    iApply (ci2a_places_inv_mono_rs). {
+      apply map_preserved_insert_r_not_in; [compute_done|].
+      apply map_preserved_insert_r_not_in; [|done].
+      clear -Hin. set_unfold. naive_solver.
+    }
+    iFrame. iApply "Hp". iSplit!.
+  - iApply (read_stack_correct with "[$]"); [done..|]. iIntros (?) "?".
+    iApply ("Hcont" with "[//] Hv").
+    iApply (ci2a_places_inv_mono_rs rs). {
+      apply map_preserved_insert_r_not_in; [compute_done|].
+      apply map_preserved_insert_r_not_in; [|done].
+      clear -Hin. set_unfold. naive_solver.
+    }
+    iFrame. iApply "Hp". iExists _. by iFrame.
+Qed.
+
+Lemma write_var_correct s s' p p' r res b n rs v av v' e vs:
+  crun s (write_var r v) = CResult s' p (CSuccess res) →
+  rs !! r = Some av →
+  ci2a_places_inv s.(s_places) s.(s_saved_registers) vs rs -∗
+  imp_val_to_asm_val v' av -∗
+  (∀ rs', ⌜s' = s⌝ -∗
+          ⌜map_scramble ("PC"::variable_registers) rs rs'⌝ -∗
+          ci2a_places_inv s.(s_places) s.(s_saved_registers) (<[v := v']>vs) rs' -∗
+          sim n true p' e s' rs') -∗
+  sim n b (p ++ p') e s rs.
+Proof.
+  unfold write_var.
+  iIntros (??) "Hp Hv Hcont". simplify_crun_eq.
+  iDestruct "Hp" as "[Hp [Hf [% [%Ha %Hbij]]]]".
+  rewrite big_sepM_delete; [|done].
+  iDestruct "Hp" as "[[% [_ Hpl]] Hp]".
+  case_match; simplify_crun_eq.
+  - iDestruct "Hpl" as %(?&?&?).
+    iApply sim_Amov. {
+      split. 2: split => ?; subst; set_solver.
+      apply: (list_elem_of_weaken variable_registers); [done| ].
+      clear. set_unfold. naive_solver.
+    }
+    simplify_map_eq'.
+    iApply ("Hcont" with "[//] [%]"). {
+      apply map_scramble_insert_r_in; [compute_done|].
+      apply map_scramble_insert_r_in; [set_unfold; naive_solver|done].
+    }
+    iApply (ci2a_places_inv_mono_rs). { apply map_preserved_insert_r_not_in; [compute_done|]. done. }
+    iFrame. rewrite (big_sepM_delete _ (s_places _)); [|done].
+    iSplit; [iSplitR "Hp"|iSplit!]; simplify_map_eq.
+    + iExists _. by iFrame.
+    + iApply (big_sepM_impl with "Hp").
+      iIntros "!>" (??[??]%lookup_delete_Some) "[%a [? Hx]]". simplify_map_eq. iExists _. iFrame.
+      case_match => //. simplify_map_eq. iDestruct "Hx" as %(?&?&?). iPureIntro. split!.
+      rewrite lookup_insert_ne //. naive_solver.
+    + apply Forall_forall => r' ?. destruct (decide (r0 = r')); [naive_solver|simplify_map_eq].
+      move: Ha => /Forall_forall. naive_solver.
+  - iApply (write_stack_correct with "[$]"); [done..|]. iIntros (?) "?".
+    iApply ("Hcont" with "[//] [%]"). { by apply map_scramble_insert_r_in; [compute_done|]. }
+    iApply (ci2a_places_inv_mono_rs rs). { apply map_preserved_insert_r_not_in; [compute_done|]. done. }
+    iFrame. rewrite (big_sepM_delete _ (s_places _)); [|done].
+    iSplit; [iSplitR "Hp"|done]; simplify_map_eq.
+    + simplify_map_eq. iExists _. iFrame.
+    + iApply (big_sepM_impl with "Hp").
+      iIntros "!>" (??[??]%lookup_delete_Some) "?". by simplify_map_eq.
+Qed.
+
+Lemma read_operand_correct e e' s s' p p' n r rs vs res K `{!ImpExprFill e' K (subst_map vs e)}:
+  crun s (read_operand r e) = CResult s' p (CSuccess res) →
+  r ∈ tmp_registers ∧ r ≠ "PC" →
+  ci2a_places_inv s.(s_places) s.(s_saved_registers) vs rs -∗
+  (∀ pc' av v,
+      let rs' := <["PC" := pc']> $ <[r := av]> rs in
+      ⌜s' = s⌝ -∗
+      imp_val_to_asm_val v av -∗
+      ci2a_places_inv s.(s_places) s.(s_saved_registers) vs rs' -∗
+      sim n true p' (expr_fill K (Val v)) s' rs') -∗
+  sim n true (p ++ p') e' s rs.
+Proof.
+  destruct ImpExprFill0; subst.
+  iIntros (??) "Hp Hcont".
+  destruct e; simplify_crun_eq.
+  - case_match; [|iApply sim_Var; typeclasses eauto with tstep].
+    iApply (read_var_correct with "Hp"); [done..|].
+    iIntros (???) "?". by iApply "Hcont".
+  - iApply sim_Amov. { set_unfold. naive_solver. }
+    iApply "Hcont"; [by simplify_map_eq|by destruct v; simplify_eq/=|].
+    iApply ci2a_places_inv_mono_rs; [|done].
+    apply map_preserved_insert_r_not_in; [compute_done|].
+    apply map_preserved_insert_r_not_in; [|done].
+    set_unfold. naive_solver.
+Qed.
+Opaque read_operand.
+
 Lemma save_r30_correct s s' p p' r n b e rs:
   crun s save_r30 = CResult s' p (CSuccess r) →
   s.(s_places) = ∅ →
@@ -477,7 +728,7 @@ Lemma save_r30_correct s s' p p' r n b e rs:
   is_Some (rs !! "R30") →
   (∀ pc' slot,
      let rs' := (<["PC":=pc']>rs) in
-     ⌜s' = s <| s_stacksize := (s_stacksize s + 1)%Z |> <|s_saved_registers := [("R30", slot)] |>⌝ -∗
+     ⌜s' = s <| s_stacksize := (s_stacksize s + 1)%N |> <|s_saved_registers := [("R30", slot)] |>⌝ -∗
      ci2a_places_inv ∅ s'.(s_saved_registers) ∅ rs' -∗
      sim n true p' e s' rs') -∗
   sim n b (p ++ p') e s rs.
@@ -488,47 +739,54 @@ Proof.
   iApply (write_stack_correct with "[$]"); [done..|]. iIntros (?) "Hs". simplify_eq.
   iApply "Hcont"; [by rewrite Hs|] => /=.
   iApply ci2a_places_inv_mono_rs. { apply map_preserved_insert_r_not_in; [compute_done|]. done. }
-  iSplit; [done|]. rewrite Hs. iSplit => /=.
-  - iSplit!.
-  - iPureIntro. apply Forall_true. by right.
+  iSplit; [done|]. rewrite Hs. iSplit! => /=.
+  - set_solver.
+  - apply Forall_true. by right.
 Qed.
 
 Lemma allocate_places_correct s ns vars s' p p' r n b e rs:
   crun s (allocate_places ns vars) = CResult s' p (CSuccess r) →
   vars ⊆+ variable_registers →
   (∀ v, v ∈ vars → v ∉ s.(s_saved_registers).*1) →
+  (∀ v n, s.(s_places) !! n = Some (PReg v) → v ∉ vars) →
   NoDup ns →
   (∀ n, n ∈ ns → s.(s_places) !! n = None) →
+  s_stacksize s = N.of_nat (length (s.(s_saved_registers)) + length (s_stack_places s.(s_places))) →
   ci2a_places_inv s.(s_places) s.(s_saved_registers) ∅ rs -∗
   (∀ rs',
      ⌜s.(s_places) ⊆ s'.(s_places)⌝ -∗
      ⌜s.(s_saved_registers) ⊆ s'.(s_saved_registers)⌝ -∗
      ⌜map_list_included ns s'.(s_places)⌝ -∗
+     ⌜s_stacksize s' = N.of_nat (length (s'.(s_saved_registers)) + length (s_stack_places s'.(s_places)))⌝ -∗
      ci2a_places_inv s'.(s_places) s'.(s_saved_registers) ∅ rs' -∗
      sim n b p' e s' rs') -∗
   sim n b (p ++ p') e s rs.
 Proof.
   elim: ns vars s s' p rs b => /=. {
-    iIntros (???????????) "? Hcont". simplify_crun_eq.
-    iApply ("Hcont" with "[//] [//] [%] [$]").
+    iIntros (?????????????) "? Hcont". simplify_crun_eq.
+    iApply ("Hcont" with "[//] [//] [%] [//] [$]").
     1: by apply map_list_included_nil. }
-  iIntros (?? IH [|v vars] ?????? Hsub Hn [??]%NoDup_cons ?) "Hp Hcont"; simplify_crun_eq.
+  iIntros (?? IH [|v vars] ?????? Hsub Hn ? [??]%NoDup_cons ?); iIntros (?) "Hp Hcont"; simplify_crun_eq.
   - rewrite -app_assoc. iApply alloc_stack_correct; [done|]. iIntros (????) "Hs". simplify_eq/=.
     iApply sim_mono_s. iIntros (???) "Hinv".
-    iSplitR; [|iSplitL "Hinv"]. 3: iApply (IH with "[Hs Hp]"); [done|done|done|done|..] => /=.
+    iSplitR; [|iSplitL "Hinv"]. 3: iApply (IH with "[Hs Hp]"); [done|done|done|set_solver|done|..] => /=.
     { done. }
     + iDestruct "Hinv" as "(?&?&?)". iFrame.
     + move => ??. apply lookup_insert_None. set_solver.
-    + iDestruct "Hp" as "[? $]". iApply big_sepM_insert; [set_solver|]. iFrame.
-      simplify_map_eq. iExists _. iFrame.
-    + iIntros (????). iApply "Hcont"; iPureIntro.
+    + rewrite /= s_stack_places_insert; [|set_solver] => /=. lia.
+    + iDestruct "Hp" as "[? [$ [$ [$ %]]]]". iSplit.
+      * iApply big_sepM_insert; [set_solver|]. iFrame.
+        simplify_map_eq. iExists _. iFrame.
+      * iPureIntro. move => ??? /lookup_insert_Some? /lookup_insert_Some?. naive_solver.
+    + iIntros (?????). iApply "Hcont"; iPureIntro.
       * etrans; [|done]. apply insert_subseteq. set_solver.
       * set_solver.
       * apply map_list_included_cons; [|done].
         apply: elem_of_weaken; [|by apply subseteq_dom].
         set_solver.
+      * done.
   - rewrite -!app_assoc. iApply alloc_stack_correct; [done|]. iIntros (????) "Hs". simplify_eq/=.
-    iApply sim_regs_included. iIntros (??).
+    iApply sim_regs_included. iIntros (?).
     move: Hsub => /submseteq_cons_l [?[Hperm Hsub]].
     have [??]: is_Some (rs !! v). {
       apply: map_list_included_is_Some.
@@ -536,36 +794,196 @@ Proof.
       rewrite Hperm. set_solver. }
     iApply (write_stack_correct with "[$]"); [done..|]. iIntros (?) "Hs". simplify_eq.
     iApply sim_mono_s. iIntros (???) "Hinv".
+    have ? : v ∉ vars. {
+      move => /(elem_of_submseteq _ _ _)/(_ Hsub).
+      apply: NoDup_cons_1_1. rewrite -Hperm. compute_done.
+    }
     iSplitR; [|iSplitL "Hinv"]. 3: iApply (IH with "[Hp Hs]"); [done|..]. all: csimpl.
     + done.
     + iDestruct "Hinv" as "(?&?&?)". iFrame.
     + rewrite Hperm. by apply submseteq_cons.
-    + move => ? Hin /=. apply not_elem_of_cons. split; [|set_unfold;naive_solver]. move => ?. subst.
-      move: Hin => /(elem_of_submseteq _ _ _)/(_ Hsub).
-      apply: NoDup_cons_1_1. rewrite -Hperm. compute_done.
+    + set_unfold; naive_solver.
+    + move => ?? /lookup_insert_Some[[??]|[??]]; set_solver.
     + done.
     + move => ??. apply lookup_insert_None. set_solver.
+    + rewrite /= s_stack_places_insert; [|set_solver] => /=. lia.
     + iApply ci2a_places_inv_mono_rs. { apply map_preserved_insert_r_not_in; [compute_done|]. done. }
-      iDestruct "Hp" as "(Hp&Hsr&%Hv)". iSplitL "Hp"; [|iSplit].
+      iDestruct "Hp" as "(Hp&Hsr&%&%Hv&%)". iSplitL "Hp"; [|repeat iSplit]; csimpl.
       * iApply big_sepM_insert; [set_solver|]. iFrame. iSplitR.
         { iExists _. simplify_map_eq. iPureIntro. split!. { rewrite Hperm. set_solver. } set_solver. }
         iApply (big_sepM_impl with "[$]"). iIntros "!>" (???) "[% [? Hp]]". iExists _. iFrame.
-        case_match => //. iDestruct "Hp" as %(?&?&?). iPureIntro. csimpl. split!. set_solver.
+        case_match => //. iDestruct "Hp" as %(?&?&?). iPureIntro. csimpl. split!. set_unfold. naive_solver.
       * simpl. iFrame. iExists _. iFrame. iPureIntro.
-        move: Hv => /Forall_forall/(_ v)[| |->//]. { rewrite Hperm. set_solver. } set_solver.
-      * iPureIntro. apply: Forall_impl; [done|]. set_solver.
-    + iIntros (????) "?". iApply sim_mono_b.
-      iApply ("Hcont" with "[%] [%] [%] [$]").
+        move: Hv => /Forall_forall/(_ v)[| |->//]. { rewrite Hperm. set_solver. }  set_unfold. naive_solver.
+      * iPureIntro. apply list_subseteq_cons_l; [|done]. rewrite Hperm. set_solver.
+      * iPureIntro. apply: Forall_impl; [done|]. set_unfold. naive_solver.
+      * iPureIntro. move => ??? /lookup_insert_Some[[??]|[??]] /lookup_insert_Some[[??]|[??]]; set_solver.
+    + iIntros (?????) "?". iApply sim_mono_b.
+      iApply ("Hcont" with "[%] [%] [%] [//] [$]").
       * etrans; [|done]. apply insert_subseteq. set_solver.
       * set_solver.
       * apply map_list_included_cons; [|done].
         apply: elem_of_weaken; [|by apply subseteq_dom].
         set_solver.
 Qed.
+
+Lemma initialize_args_correct s xs s' p p' r n e rs vs vm:
+  crun s (initialize_args xs) = CResult s' p (CSuccess r) →
+  length xs = length vs →
+  NoDup xs →
+  ([∗ list] i↦v∈vs, ∃ r av, ⌜args_registers !! (0 + i)%nat = Some r⌝ ∗ ⌜rs !! r = Some av⌝ ∗ imp_val_to_asm_val v av) -∗
+  ci2a_places_inv s.(s_places) s.(s_saved_registers) vm rs -∗
+  (∀ rs',
+     ⌜s' = s⌝ -∗
+     ⌜map_scramble ("PC"::variable_registers) rs rs'⌝ -∗
+     ci2a_places_inv s'.(s_places) s'.(s_saved_registers) (list_to_map (zip xs vs) ∪ vm) rs' -∗
+     sim n true p' e s' rs') -∗
+  sim n true (p ++ p') e s rs.
+Proof.
+  unfold initialize_args.
+  elim: xs vs vm s s' p rs 0%nat => /=. {
+    move => [|//] ?????????. simplify_crun_eq.
+    iIntros "_ Hp Hcont". iApply "Hcont"; [done..|]. by rewrite left_id_L.
+  }
+  move => ?? IH [//|??] ??????? /=[?] /NoDup_cons[??]. simplify_crun_eq.
+  rewrite Nat.add_0_r. iIntros "[[% [% [% [% ?]]]] Hl] Hp Hcont". simplify_eq.
+  rewrite -!app_assoc /=.
+  iApply (write_var_correct with "[$] [$]"); [done..|].
+  iIntros (?? Hrs) "Hp". simplify_eq.
+  iApply (IH with "[Hl] Hp"). { apply cbind_success. split!; [done..|]. by rewrite app_nil_r. }
+  { done. } { done. }
+  { setoid_rewrite Nat.add_succ_l. setoid_rewrite Nat.add_succ_r.
+    iApply (big_sepL_impl with "[$]"). iIntros "!>" (???) "[% [% [%Hlookup [% ?]]]]".
+    iSplit!; [done| |done].
+    etrans; [symmetry; apply: Hrs|done]. move: Hlookup => /(elem_of_list_lookup_2 _ _ _).
+    clear. set_unfold. naive_solver.
+  }
+  iIntros (???) "Hp".
+  iApply "Hcont"; [done|iPureIntro;by etrans|].
+  rewrite -insert_union_l -insert_union_r; [done|].
+  apply not_elem_of_list_to_map_1. rewrite fst_zip //. lia.
+Qed.
+
+Lemma translate_expr_op_correct s s' p p' n e rs vs res K:
+  crun s (translate_expr_op e) = CResult s' p (CSuccess res) →
+  ci2a_places_inv s.(s_places) s.(s_saved_registers) vs rs -∗
+  (∀ rs' vs' av v,
+      ⌜rs' !! "R0" = Some av⌝ -∗
+      ⌜s' = s⌝ -∗
+      imp_val_to_asm_val v av -∗
+      ci2a_places_inv s.(s_places) s.(s_saved_registers) vs' rs' -∗
+      sim n true p' (expr_fill K (Val v)) s' rs') -∗
+  sim n true (p ++ p') (expr_fill K (subst_map vs e)) s rs.
+Proof.
+  iIntros (?) "Hp Hcont".
+  destruct e; simplify_crun_eq.
+  - iApply (read_operand_correct (Var _) with "Hp"); [typeclasses eauto with tstep|done|compute_done|].
+    iIntros (????) "? Hp".
+    iApply ("Hcont" with "[] [//] [$] Hp"). by simplify_map_eq.
+  - iApply (read_operand_correct (Val _) with "Hp"); [typeclasses eauto with tstep|done|compute_done|].
+    iIntros (????) "? Hp".
+    iApply ("Hcont" with "[] [//] [$] Hp"). by simplify_map_eq.
+  - rewrite -!app_assoc.
+    iApply sim_regs_included. iIntros (?).
+    iApply (read_operand_correct with "Hp"); [typeclasses eauto with tstep|done|compute_done|].
+    iIntros (?? v1 ?) "? Hp". simplify_eq/=.
+    iApply (read_operand_correct with "Hp"); [typeclasses eauto with tstep|done|compute_done|].
+    iIntros (?? v2 ?) "? Hp". simplify_eq/=.
+    iIntros (???? Hins) "Hrf Hinv".
+    iSatStop. tstep_s => ??.
+    case_match; simplify_crun_eq; destruct v1 as [|b1|], v2 as [|b2|] => //; simplify_eq/=.
+    all: iSatStart; iDestruct!; iSatStop.
+    all: tstep_i => ??; simplify_map_eq'.
+    all: move: Hins => /deep_to_asm_instrs_cons_inv[??]; simplify_map_eq.
+    all: tstep_i; simplify_map_eq'; split!; [apply: map_list_included_is_Some; [done|compute_done]|].
+    all: tstep_i; simplify_map_eq'; split!.
+    all: iSatStart.
+    all: try iDestruct select (i2a_heap_shared _ _) as "#Hs".
+    all: iApply (to_sim with "[Hcont Hp] [] Hrf"); [|by simplify_map_eq'|
+      iDestruct "Hinv" as "($&$&?)";
+      iApply ci2a_regs_inv_mono_insert; [compute_done|];
+      iApply ci2a_regs_inv_mono_insert; [compute_done|done]].
+    all: iApply "Hcont"; [by simplify_map_eq|done|simpl|
+      iApply ci2a_places_inv_mono_rs; [|done];
+      apply map_preserved_insert_r_not_in; [compute_done|];
+      by apply map_preserved_insert_r_not_in; [compute_done|]].
+    + done.
+    + iExists _ => /=. iFrame "#". iPureIntro. lia.
+    + done.
+    + iPureIntro. destruct b1, b2 => //.
+    + done.
+    + done.
+  - rewrite -!app_assoc.
+    iApply (read_operand_correct with "Hp"); [typeclasses eauto with tstep|done|compute_done|].
+    iIntros (?? v ?) "? Hp". simplify_eq/=.
+    admit.
+  - rewrite -!app_assoc.
+    iApply (read_operand_correct with "Hp"); [typeclasses eauto with tstep|done|compute_done|].
+    iIntros (?? v1 ?) "? Hp". simplify_eq/=.
+    iApply (read_operand_correct with "Hp"); [typeclasses eauto with tstep|done|compute_done|].
+    iIntros (?? v2 ?) "? Hp". simplify_eq/=.
+    admit.
+  - rewrite -!app_assoc.
+    admit.
+Admitted.
+Opaque translate_expr_op.
+
+Lemma translate_expr_correct s s' p p' n e rs vs res K:
+  crun s (translate_expr e) = CResult s' p (CSuccess res) →
+  ci2a_places_inv s.(s_places) s.(s_saved_registers) vs rs -∗
+  (∀ rs' vs' av v,
+      ⌜rs' !! "R0" = Some av⌝ -∗
+      ⌜s' = s⌝ -∗
+      imp_val_to_asm_val v av -∗
+      ci2a_places_inv s.(s_places) s.(s_saved_registers) vs' rs' -∗
+      sim n true p' (expr_fill K (Val v)) s' rs') -∗
+  sim n true (p ++ p') (expr_fill K (subst_map vs e)) s rs.
+Proof.
+  elim: e vs s s' p rs => *; simplify_crun_eq.
+Admitted.
+
+Lemma restore_callee_save_registers_correct s s' p p' r n e rs:
+  crun s restore_callee_save_registers = CResult s' p (CSuccess r) →
+  s.(s_saved_registers).*1 ⊆ "R30"::variable_registers →
+  ([∗ list] r ∈ s.(s_saved_registers), ∃ v : Z, ⌜pf_rsold !! r.1 = Some v⌝ ∗ stack_slot r.2 v) -∗
+  (∀ rs',
+     ⌜s' = s⌝ -∗
+     ⌜map_scramble ("PC"::s.(s_saved_registers).*1) rs rs'⌝ -∗
+     ⌜Forall (λ r, rs' !! r.1 = Some (pf_rsold !!! r.1)) s.(s_saved_registers)⌝ -∗
+     ([∗ list] r ∈ s.(s_saved_registers), ∃ v : Z, stack_slot r.2 v) -∗
+     sim n true p' e s' rs') -∗
+  sim n true (p ++ p') e s rs.
+Proof.
+  unfold restore_callee_save_registers.
+  move: 0%nat => n'.
+  iIntros (? Hsub ) "Hsr Hcont". simplify_crun_eq.
+  rewrite -!app_assoc/=.
+  rename select (crun _ _ = _) into Hrun.
+  match type of Hrun with | _ = CResult _ ?x (CSuccess ?r') => rename x into p; rename r' into res end.
+  iInduction (s_saved_registers s) as [|[r ?] ?] "IH" forall (rs p res n' Hrun); simplify_crun_eq. 1: by iApply "Hcont".
+  rewrite -!app_assoc/=.
+  iDestruct "Hsr" as "[[% [% Hs]] Hsr]".
+  iApply (read_stack_correct with "Hs"); [done| |]. { set_unfold; naive_solver. }
+  iIntros (?) "Hs". simplify_eq.
+  iApply ("IH" with "[%] [//] Hsr"); [set_solver|].
+  iIntros (?? Hrs Hall) "?".
+  iApply "Hcont"; try iPureIntro.
+  - done.
+  - etrans. 2: { apply: map_scramble_mono; [done|]. set_solver. }
+    apply map_scramble_insert_r_in; [set_solver|].
+    apply map_scramble_insert_r_in; [set_solver|]. done.
+  - econs; [|done] => /=.
+    destruct (decide (r ∈ l.*1)) as [[?[??]]%elem_of_list_fmap|].
+    + move: Hall => /Forall_forall. naive_solver.
+    + simplify_map_eq'. etrans; [symmetry; apply: Hrs; set_solver|].
+      rewrite lookup_insert_ne; [| set_solver]. by simplify_map_eq.
+  - iFrame. iExists _. iFrame.
+Qed.
+
 End proof.
 
 Lemma sim_intro s dins rs mem ins ins_dom fns_dom f2i n b e h fns cs lr rf P:
-  let H := Build_ProofFixedValues (rs !!! "SP") ins fns cs rs in
+  let H := Build_ProofFixedValues (rs !!! "SP") ins fns cs rs f2i in
   deep_to_asm_instrs (rs !!! "PC") dins = ins →
   ins_dom = dom _ ins →
   fns_dom = dom _ fns →
@@ -586,36 +1004,99 @@ Lemma pass_correct a f2i f fn s' dins ins :
   crun (initial_state f2i) (pass fn) = CResult s' dins (CSuccess tt) →
   ins = deep_to_asm_instrs a dins →
   f2i !! f = Some a →
+  NoDup (fn.(fd_args)) →
   trefines (MS asm_module (initial_asm_state ins))
            (MS (imp_to_asm (dom _ ins) {[f]} f2i imp_module) (initial_imp_to_asm_state imp_module
              (initial_imp_state (<[f := fn]> ∅)))).
 Proof.
-  move => Hrun ? Ha.
+  move => Hrun ? Ha ?.
   apply imp_to_asm_proof; [done|set_solver|].
-  move => n i rs mem K f' fn' avs vs h cs pc ret rf rc amem ih lr Hpc Hins Hf ? Hsat Hinv Hargs Hlen Hlr Hcall Hret.
+  move => n i rs mem K f' fn' avs vs h cs pc ret rf rc lr Hpc Hins Hf ? Hsat Hargs Hlen Hlr Hcall Hret.
   move: Hf. rewrite lookup_insert_Some lookup_empty => ?. destruct_all?; simplify_map_eq.
-  move: Hinv => [?[??]].
   move: Hargs => [?[?[??]]].
 
   apply: (sim_intro (initial_state f2i)).
   1: by simplify_map_eq'. 1: done. 1: set_solver. 1: done. {
-    iSatMono. iIntros "(Hmem&Hheap&Hshare&Hvals&?&?)". iFrame.
-    iSplitL "Hmem Hheap Hshare". 2: iAccu.
-    iSplitL "Hmem" => /=; [|iSplitL].
-    - iExists _. iFrame. iPureIntro. by rewrite Z.sub_0_r.
-    - iExists _. by iFrame.
-    - iPureIntro => /=. rewrite lookup_lookup_total; [done|].
-      apply: (map_list_included_is_Some saved_registers); [done|compute_done].
+    iSatMono. iIntros "(Hmem&Hheap&Hvals&?&?)". iFrame => /=. rewrite Z.sub_0_r. iFrame.
+    iSplitR. 2: iAccu.
+    iPureIntro => /=. rewrite /touched_registers map_list_included_app lookup_lookup_total; [done|].
+    apply: (map_list_included_is_Some saved_registers); [done|compute_done].
   }
   iSatClear.
   iIntros "(Hvals&Hrc)".
   unfold pass in Hrun. simplify_crun_eq.
+  rename x3 into s.
 
   iApply save_r30_correct; [done..|]. iIntros (???) "Hp". simplify_eq/=.
   iApply (allocate_places_correct with "[Hp]").
-  { done. } { done. } { set_solver. } { apply NoDup_remove_dups. }
-  { set_solver. } { done. }
-  iIntros (????) "Hpl". simplify_eq/=.
+  { done. } { done. } { set_solver. } { naive_solver. } { apply NoDup_remove_dups. }
+  { set_solver. } { done. } { done. }
+  iIntros (?????) "Hpl". simplify_eq/=.
+  iApply (initialize_args_correct with "[Hvals] Hpl").
+  { done. } { done. } { done. }
+  { admit. }
+  iIntros (???) "Hpl". simplify_eq.
+  iApply (move_sp_correct); [done|].
+  iIntros (???). simplify_eq.
+  rewrite subst_l_subst_map // right_id_L.
+  iApply (translate_expr_correct with "[Hpl]"); [done| |].
+  { iApply ci2a_places_inv_mono_rs; [|done].
+    apply map_preserved_insert_r_not_in; [compute_done|].
+    apply map_preserved_insert_r_not_in; [compute_done|done]. }
+  iIntros (??????) "Hv Hp". simplify_eq.
+  iApply move_sp_correct; [done|].
+  iIntros (???). simplify_eq/=.
+  iDestruct "Hp" as "(Hpl&Hsr&%Hsub&%Hall&_)".
+  iApply (restore_callee_save_registers_correct with "[Hsr]"); [done..|] => /=.
+  iIntros (?? Hrs2 Hallsr) "Hsr".
+
+  clear Hins.
+  iIntros (???? Hins) "? (Hmem&Hh&(%Hsp1&%Hsp2&%&%&%))".
+  iSatStop.
+  tstep_i => ??. simplify_map_eq.
+  move: Hins => /deep_to_asm_instrs_cons_inv[??]. simplify_map_eq'.
+  tstep_i. split!.
+  rewrite dom_insert_L dom_empty_L right_id_L.
+  eapply Hret.
+  - simplify_map_eq'. f_equal. eapply lookup_total_correct.
+    move: Hallsr => /Forall_forall/(_ ("R30", slot)) ->. 2: set_unfold; naive_solver.
+    by simplify_map_eq'.
+  - iSatMonoBupd. simplify_map_eq'. iFrame.
+    iApply (i2a_mem_delete_big
+              ((λ slot, rs !!! "SP" - Z.of_N slot - 1) <$> ((s_saved_registers s).*2 ++ s_stack_places s.(s_places)))
+             with "Hmem").
+    + lia.
+    + apply Forall_forall => ? /elem_of_list_fmap[?[??]]. subst. lia.
+    + rewrite fmap_length app_length fmap_length. lia.
+    +
+
+  - unfold imp_to_asm_ret. simplify_map_eq'. split!.
+    + apply lookup_total_correct. etrans; [symmetry; apply: Hrs2; set_unfold; naive_solver |].
+      by simplify_map_eq.
+    + apply map_list_included_insert. apply: map_list_included_mono; [done|]. compute_done.
+    + apply map_preserved_insert_r_not_in; [compute_done|].
+      have ->: saved_registers = variable_registers ++ ["SP"] by compute_done.
+      apply map_preserved_app. split. 2: { move => ?. set_unfold => ?. naive_solver congruence. }
+      move => r Hr.
+      destruct (decide (r ∈ (s_saved_registers s).*1)) as [[?[? Hin]]%elem_of_list_fmap|?].
+      * move: Hallsr Hin => /Forall_forall/[apply]?. subst. etrans; [done|]. symmetry.
+        apply lookup_lookup_total. apply: map_list_included_is_Some; [done|].
+        apply: list_elem_of_weaken; [done|]. clear. set_solver.
+      * move: Hall (Hr) => /Forall_forall/[apply] -[//| ->].
+        symmetry. etrans; [|apply: Hrs2; set_unfold; naive_solver].
+        rewrite !lookup_insert_ne //; set_unfold; naive_solver.
+  - by apply map_scramble_insert_r_in; [compute_done|].
+
+
+
+map_list_included_insert. apply: map_list_included_mono; [done|]. compute_done.
+
+split
+    admit.
+
+
+  tstep_i. split!; simplify_map_eq'; [done|].
+  iSatStart.
 
   (* move: (fd_args fn') => xs. *)
   (* move: (fd_body fn') Hrun => e. *)
@@ -634,28 +1115,3 @@ Proof.
 Abort.
 
 End ci2a_codegen.
-(*
-optimizations:
-
-fn f() :=
-  local x
-  x ← 1;
-  g(!x + !x);
-  x ← 2;
-  return !x
-
-optimize to:
-
-fn f() :=
-  let x := 1;
-  g(x + x);
-  let x := 2;
-  return x
-
-1 + 1 → 2
-
-if 1 then e1 else e2
-->
-e1
-
-*)
