Notes.md
@@ -4,11 +4,24 @@
   - Maybe let x := Alloc 1 in x ← 1; let y = int_to_ptr(ptr_to_int(x)) in let r := !y in Free(y); Return r
     - refines Return 1
 - [ ] Define pure_i2a.imp_to_asm
-- [ ] Prove vertical compositionality of pure_i2a.imp_to_asm and pure_bij.heap_bij
-  - Should be easier than vertical compositionality for heap_bij since
-    e.g. we don't need heap_in_bij for middle module to outside
-- [ ] Prove equivalence of pure_i2a.imp_to_asm and imp_to_asm
-- [ ] Prove equivalence of pure_bij.heap_bij and heap_bij
+- [ ] prove vertical compositionality
+  - Plan A: prove vertical compositionality directly on ownership based prepost
+    - [ ] Add [∗ map] ps\mapsto pi \in hb_shared bij, shared ps pi to
+          invariant of heap_bij. This ensures that all shared locations are shared persistently.
+    - [ ] Use invariant when proving vertical compositionality:
+          Additional locations we own in the spec + locations we own
+          in the target cover all private locations. This means that
+          we can replay all modifications that the env does in the
+          source in the target because we own all locations that the
+          env could modify in the source and vice versa. Might need
+          some additional trickery for i2a (maybe subtract all
+          addresses that correspond to shared locations?)
+  - [ ] Prove vertical compositionality of pure_i2a.imp_to_asm and
+        pure_bij.heap_bij
+    - Should be easier than vertical compositionality for heap_bij since
+      e.g. we don't need heap_in_bij for middle module to outside
+  - [ ] Prove equivalence of pure_i2a.imp_to_asm and imp_to_asm
+  - [ ] Prove equivalence of pure_bij.heap_bij and heap_bij
 - [ ] Add ghost state for f2i and add values of f2i to initial ownership
 - [ ] Add fnptrs to imp (should be easy when one has ghost state for f2i)
 - [ ] Add global variables
